theories/sim/instance.v
@@ -3,11 +3,11 @@ From stbor.sim Require Export local invariant.
 
 Notation "r ⊨{ n , fs , ft } ( es , σs ) ≥ ( et , σt ) : Φ" :=
   (sim_local_body wsat vrel fs ft r n%nat es%E σs et%E σt Φ)
-  (at level 70, format "'[hv' r  '/' ⊨{ n , fs , ft } '/  ' '[ ' ( es ,  '/' σs ) ']' '/' ≥  '/  ' '[ ' ( et ,  '/' σt ) ']'  '/' :  Φ ']'").
+  (at level 70, format "'[hv' r  '/' ⊨{ n , fs , ft }  '/  ' '[ ' ( es ,  '/' σs ) ']'  '/' ≥  '/  ' '[ ' ( et ,  '/' σt ) ']'  '/' :  Φ ']'").
 
-Notation "⊨{ fs , ft } f1 ≥ᶠ f2" :=
+Notation "⊨ᶠ{ fs , ft } f1 ≥ f2" :=
   (sim_local_fun wsat vrel fs ft end_call_sat f1 f2)
-  (at level 70, format "⊨{ fs , ft }  f1  ≥ᶠ  f2").
+  (at level 70, f1, f2 at next level, format "⊨ᶠ{ fs , ft }  f1  ≥  f2").
 
 Lemma sim_body_result fs ft r n es et σs σt Φ :
   (✓ r → Φ r n es σs et σt : Prop) →
