theories/sim/simple.v
@@ -1,0 +1,27 @@
+(** A simpler simulation relation that hides the physical state.
+Useful whenever the resources we own are strong enough to carry us from step to step.
+
+When your goal is simple, to make it stateful just do [intros σs σt].
+To go the other direction, [apply sim_simplify]. Then you will likely
+want to clean some stuff from your context.
+*)
+
+From stbor.sim Require Export instance.
+
+Definition sim_simple fs ft r n es et Φ : Prop :=
+  ∀ σs σt, r ⊨{ n , fs , ft } ( es , σs ) ≥ ( et , σt ) : Φ.
+
+Notation "r ⊨ˢ{ n , fs , ft } es '≥' et : Φ" :=
+  (sim_simple fs ft r n%nat es%E et%E Φ)
+  (at level 70, es, et at next level,
+   format "'[hv' r  '/' ⊨ˢ{ n , fs , ft }  '/  ' '[ ' es ']'  '/' ≥  '/  ' '[ ' et ']'  '/' :  Φ ']'").
+
+Lemma sim_fun_simple1 n fs ft (esf etf: function) Φ :
+  length (esf.(fun_b)) = 1%nat →
+  length (etf.(fun_b)) = 1%nat →
+  (∀ es et vs vt r, vrel r vs vt →
+   subst_l (esf.(fun_b)) [Val vs] (esf.(fun_e)) = Some es →
+   subst_l (etf.(fun_b)) [Val vt] (etf.(fun_e)) = Some et →
+   r ⊨ˢ{n,fs,ft} es ≥ et : Φ) →
+  ⊨ᶠ{fs,ft} esf ≥ etf.
+Abort.
